ConLeche/Model/Inductives/FixLeafOk.lean
@@ -60,9 +60,9 @@ theorem AnnotValid_congr_noBVar :
     intro P σ σ' h hag
     rw [AnnotValid_letE, AnnotValid_letE, ihT h.1 hag, ihv h.2.1 hag,
       ihb h.2.2 (agreeOff_cons_of hag (interp_congr_noBVar v h.2.1 hag))]
-  | eqE T a b ihT iha ihb =>
+  | eqE a b iha ihb =>
     intro P σ σ' h hag
-    rw [AnnotValid, AnnotValid, iha h.2.1 hag, ihb h.2.2 hag]
+    rw [AnnotValid, AnnotValid, iha h.1 hag, ihb h.2 hag]
   | fst e ihe =>
     intro P σ σ' h hag
     rw [AnnotValid_fst, AnnotValid_fst, ihe h hag]
