ConLeche/Term/Const.lean
@@ -118,7 +118,7 @@ def BConst.type : BConst → List Nat → Term
     .pi (.pi (.bvar 2) (.bvar 1)) <|
     .pi (.pi (.bvar 3) (.pi (.bvar 4)
           (.pi (mkAppN (.bvar 4) [.bvar 1, .bvar 0])
-            (.eqE (.bvar 4) (.app (.bvar 3) (.bvar 2))
+            (.eqE (.app (.bvar 3) (.bvar 2))
               (.app (.bvar 3) (.bvar 1)))))) <|
     .pi (quotT u (.bvar 4) (.bvar 3)) <|
     .bvar 3
@@ -137,15 +137,14 @@ def BConst.type : BConst → List Nat → Term
     .pi (.bvar 1) <|
     .pi (.bvar 2) <|
     .pi (mkAppN (.bvar 2) [.bvar 1, .bvar 0]) <|
-    .eqE (quotT u (.bvar 4) (.bvar 3))
-      (quotMkT u (.bvar 4) (.bvar 3) (.bvar 2))
+    .eqE (quotMkT u (.bvar 4) (.bvar 3) (.bvar 2))
       (quotMkT u (.bvar 4) (.bvar 3) (.bvar 1))
   | .propext, _ =>
     -- `∀ (A B : Prop), (A → B) → (B → A) → A = B`
     .pi (.sort 0) <| .pi (.sort 0) <|
     .pi (.pi (.bvar 1) (.bvar 1)) <|
     .pi (.pi (.bvar 1) (.bvar 3)) <|
-    .eqE (.sort 0) (.bvar 3) (.bvar 2)
+    .eqE (.bvar 3) (.bvar 2)
   | .choice, us =>
     let u := lv us 0
     -- `∀ (A : Sort u), ¬¬A → A`
